revm: beginning of links for contract instructions

CoqOfRust/alloc/links/boxed.v
@@ -1,5 +1,7 @@
 Require Import CoqOfRust.CoqOfRust.
 Require Import links.M.
+Require Import alloc.boxed.
+Require Import alloc.links.alloc.
 
 Module Box.
   Record t {T A : Set} : Set := {
@@ -14,4 +16,30 @@ Module Box.
       Ty.apply (Ty.path "alloc::boxed::Box") [] [ Φ T; Φ A ];
     φ := to_value;
   }.
+
+  Definition of_ty (T_ty A_ty : Ty.t) :
+    OfTy.t T_ty ->
+    OfTy.t A_ty ->
+    OfTy.t (Ty.apply (Ty.path "alloc::boxed::Box") [] [ T_ty; A_ty ]).
+  Proof.
+    intros [T] [A].
+    eapply OfTy.Make with (A := t T A).
+    now subst.
+  Defined.
+  Smpl Add eapply of_ty : of_ty.
 End Box.
+
+Module Impl_Box.
+  Definition Self (T : Set) : Set :=
+    Box.t T Global.t.
+
+  Instance run_new (T : Set) `{Link T} (x : T) :
+    Run.Trait
+      (boxed.Impl_alloc_boxed_Box_T_alloc_alloc_Global.new (Φ T)) [] [] [ φ x ]
+      (Self T).
+  Proof.
+    constructor.
+    run_symbolic.
+  Admitted.
+End Impl_Box.
+Export Impl_Box.
