CoqOfRust/revm/revm_interpreter/instructions/contract/links/call_helpers.v
@@ -1,0 +1,73 @@
+Require Import CoqOfRust.CoqOfRust.
+Require Import CoqOfRust.links.M.
+Require Import alloy_primitives.bytes.links.mod.
+Require Import alloy_primitives.links.aliases.
+Require Import core.links.option.
+Require Import core.ops.links.range.
+Require Import revm.revm_context_interface.links.journaled_state.
+Require Import revm.revm_interpreter.instructions.contract.call_helpers.
+Require Import revm.revm_interpreter.links.interpreter.
+Require Import revm.revm_interpreter.links.interpreter_types.
+
+(*
+pub fn get_memory_input_and_out_ranges(
+    interpreter: &mut Interpreter<impl InterpreterTypes>,
+) -> Option<(Bytes, Range<usize>)>
+*)
+Instance run_get_memory_input_and_out_ranges
+  {WIRE : Set} `{Link WIRE}
+  {WIRE_types : InterpreterTypes.Types.t} `{InterpreterTypes.Types.AreLinks WIRE_types}
+  (run_InterpreterTypes_for_WIRE : InterpreterTypes.Run WIRE WIRE_types)
+  (interpreter : Ref.t Pointer.Kind.MutRef (Interpreter.t WIRE WIRE_types)) :
+  Run.Trait
+    instructions.contract.call_helpers.get_memory_input_and_out_ranges
+    [] [Φ WIRE] [φ interpreter]
+    (option (Bytes.t * Range.t Usize.t)).
+Proof.
+  constructor.
+Admitted.
+
+(*
+pub fn resize_memory(
+    interpreter: &mut Interpreter<impl InterpreterTypes>,
+    offset: U256,
+    len: U256,
+) -> Option<Range<usize>>
+*)
+Instance run_resize_memory
+  {WIRE : Set} `{Link WIRE}
+  {WIRE_types : InterpreterTypes.Types.t} `{InterpreterTypes.Types.AreLinks WIRE_types}
+  (run_InterpreterTypes_for_WIRE : InterpreterTypes.Run WIRE WIRE_types)
+  (interpreter : Ref.t Pointer.Kind.MutRef (Interpreter.t WIRE WIRE_types))
+  (offset len : aliases.U256.t) :
+  Run.Trait
+    instructions.contract.call_helpers.resize_memory
+    [] [Φ WIRE] [φ interpreter; φ offset; φ len]
+    (option (Range.t Usize.t)).
+Proof.
+  constructor.
+Admitted.
+
+(*
+pub fn calc_call_gas(
+    interpreter: &mut Interpreter<impl InterpreterTypes>,
+    account_load: AccountLoad,
+    has_transfer: bool,
+    local_gas_limit: u64,
+) -> Option<u64>
+*)
+Instance run_calc_call_gas
+  {WIRE : Set} `{Link WIRE}
+  {WIRE_types : InterpreterTypes.Types.t} `{InterpreterTypes.Types.AreLinks WIRE_types}
+  (run_InterpreterTypes_for_WIRE : InterpreterTypes.Run WIRE WIRE_types)
+  (interpreter : Ref.t Pointer.Kind.MutRef (Interpreter.t WIRE WIRE_types))
+  (account_load : AccountLoad.t)
+  (has_transfer : bool)
+  (local_gas_limit : U64.t) :
+  Run.Trait
+    instructions.contract.call_helpers.calc_call_gas
+    [] [Φ WIRE] [φ interpreter; φ account_load; φ has_transfer; φ local_gas_limit]
+    (option U64.t).
+Proof.
+  constructor.
+Admitted.
